functional_programming/functional_programming_5.lean
@@ -1,0 +1,130 @@
+-- Mapping on a Tree
+
+inductive BinTree (α : Type) where
+  | leaf : BinTree α
+  | branch : BinTree α → α → BinTree α → BinTree α
+deriving Repr
+
+def eqBinTree [BEq α] : BinTree α → BinTree α → Bool
+  | BinTree.leaf, BinTree.leaf =>
+    true
+  | BinTree.branch l x r, BinTree.branch l2 x2 r2 =>
+    x == x2 && eqBinTree l l2 && eqBinTree r r2
+  | _, _ =>
+    false
+
+instance [BEq α] : BEq (BinTree α) where
+  beq := eqBinTree
+
+def hashBinTree [Hashable α] : BinTree α → UInt64
+  | BinTree.leaf =>
+    0
+  | BinTree.branch left x right =>
+    mixHash 1 (mixHash (hashBinTree left) (mixHash (hash x) (hashBinTree right)))
+
+instance [Hashable α] : Hashable (BinTree α) where
+  hash := hashBinTree
+
+def BinTree.mapM [Monad m] (f : α → m β) : BinTree α → m (BinTree β) 
+  | leaf => pure BinTree.leaf
+  | branch l v r => f v >>= fun x => BinTree.mapM f l >>= fun y => BinTree.mapM f r >>= fun z => pure (BinTree.branch y x z)
+
+def tree := BinTree.branch (BinTree.branch BinTree.leaf 4 BinTree.leaf) 5 (BinTree.branch BinTree.leaf 12 (BinTree.branch BinTree.leaf 50 BinTree.leaf)) 
+
+-- def test : BinTree Nat -> Nat
+--   | BinTree.leaf => 0 
+--   | BinTree.branch l v r => 0 
+
+#eval BinTree.mapM (m := Id) (fun x => x) tree
+
+-- The Option Monad Contract
+
+-- correct 
+instance : Monad Option where
+  pure x := some x
+  bind opt next :=
+    match opt with
+    | none => none
+    | some x => next x
+
+-- wrong 
+instance : Monad Option where
+  pure x := some x
+  bind opt next := none
+--  bind (pure v) f should be the same as f v
+
+inductive Many (α : Type) where
+  | none : Many α
+  | more : α → (Unit → Many α) → Many α
+
+def Many.one (x : α) : Many α := Many.more x (fun ⟨⟩ => Many.none)
+
+
+-- Checking Contracts
+-- Check the monad contract for State σ and Except ε.
+
+
+
+
+instance : Monad (Except ε) where
+  pure x := Except.ok x
+  bind attempt next :=
+    match attempt with
+    | Except.error e => Except.error e
+    | Except.ok x => next x
+
+-- Except.bind (Except.pure v) f
+-- Except.bind (Except.ok v) f
+-- f v
+
+-- Except.bind v Except.pure == v
+-- attempt = v
+-- next == pure 
+-- if v == error => v 
+-- if v == ok => pure ok => v
+
+-- bind (bind v f) g == bind v (fun x => bind (f x) g)
+-- Except.bind (Except.bind v f) g
+-- 
+
+def State (σ : Type) (α : Type) : Type :=
+  σ → (σ × α)
+
+instance : Monad (State σ) where
+  pure x := fun s => (s, x)
+  bind first next :=
+    fun s =>
+      let (s', x) := first s
+      next x s'
+
+-- bind (pure v) f
+-- bind (fun s => (s,v)) f 
+-- first = (fun s => (s,v)), next = f 
+-- fun y => s' = s and x = v
+-- f x s' 
+
+-- Readers with Failure
+
+def Reader (ρ : Type) (α : Type) : Type := ρ → α
+
+def read : Reader ρ ρ := fun env => env
+
+def Reader.pure (x : α) : Reader ρ α := fun _ => x
+
+def Reader.bind (result : Reader ρ α) (next : α → Reader ρ β) : Reader ρ β :=
+  fun env => next (result env) env
+
+def ReaderOption (ρ : Type) (α : Type) : Type := ρ → Option α
+
+def ReaderOption.pure (x : α) : ReaderOption ρ (Option α) := fun _ => some x
+
+-- def ReaderOption.bind (result : ReaderOption ρ (Option α)) (next : α → ReaderOption ρ β) : ReaderOption ρ β :=
+--   fun env => next (result env) env
+
+def ReaderExcept (ε : Type) (ρ : Type) (α : Type) : Type := ρ → Except ε α
+
+abbrev Env : Type := List (String × (Int → Int → Int))
+
+def exampleEnv : Env := [("max", max), ("mod", (· % ·))]
+
+#check ReaderOption.pure 6
