theorem_proving/exercises_chapter_8.lean
@@ -1,0 +1,226 @@
+namespace Hidden
+-- 1
+inductive Nat where 
+  | zero : Nat 
+  | succ : Nat → Nat 
+deriving Repr 
+
+def add : Nat → Nat → Nat 
+  | Nat.zero, k => k
+  | Nat.succ n, k => Nat.succ (add n k)
+
+#eval add (Nat.succ (Nat.succ Nat.zero)) (Nat.succ Nat.zero)
+
+def mul : Nat → Nat → Nat 
+  | Nat.zero, _ => Nat.zero
+  | Nat.succ n, k => add k (mul n k)
+
+#eval mul (Nat.succ (Nat.succ Nat.zero)) (Nat.succ (Nat.succ Nat.zero))
+
+def pow (n m : Nat) : Nat := 
+  match m with 
+  | Nat.zero => Nat.succ Nat.zero 
+  | Nat.succ m => mul n (pow n m)
+
+#eval pow (Nat.succ (Nat.succ Nat.zero)) (Nat.succ (Nat.succ (Nat.succ Nat.zero)))
+
+--2
+inductive List (α : Type u) where
+  | nil  : List α
+  | cons : α → List α → List α
+deriving Repr 
+
+notation  (priority := high) "[" "]" => List.nil   -- `[]`
+infixr:67 (priority := high) " :: "  => List.cons  -- `a :: as`
+
+-- as a warm-up exercise, let's define concatenation of two lists
+def append (as bs : List α) : List α := 
+  match as with 
+  | [] => bs 
+  | x :: xs => x :: (append xs bs)
+
+infixl:65 (priority := high) " ++ " => append
+
+def reverse (xs : List α) : List α := 
+  match xs with 
+  | List.nil => List.nil
+  | List.cons x xs => (reverse xs) ++ (List.cons x List.nil)
+
+@[simp]theorem append_nil (xs: List α) : reverse (xs ++ []) = [] ++ reverse xs := by 
+  induction xs 
+  . case nil => rfl 
+  . case cons x xs h => simp [h, append, reverse]
+
+@[simp]theorem nil_append (xs: List α) : reverse ([] ++ xs) = reverse xs ++ [] := by 
+  induction xs 
+  . case nil => rfl 
+  . case cons x xs h => 
+    rw [reverse]
+    sorry
+    -- simp [h, append, reverse]
+
+
+theorem reverse_append (xs : List α) (ys : List α) : reverse (xs ++ ys) = reverse ys ++ reverse xs := by
+  induction xs
+  . case nil => sorry
+  . case cons x xs => 
+    sorry
+
+
+#eval reverse (List.cons 1 (List.cons 2 (List.cons 3 List.nil)))
+
+theorem double_reverse (xs : List α) : reverse (reverse xs) = xs := by
+  induction xs
+  . case nil => rfl
+  . case cons x xs h => 
+    rw [reverse]
+    sorry
+    -- simp [h] 
+    -- simp [reverse, append]
+
+    -- simp_all [reverse, h, append]
+
+-- 3   
+
+
+end Hidden 
+
+-- 4 
+
+inductive Vector (α : Type u) : Nat → Type u
+  | nil  : Vector α 0
+  | cons : α → {n : Nat} → Vector α n → Vector α (n+1)
+deriving Repr
+
+namespace Vector
+
+def v1 := Vector.cons 5 (Vector.cons 0 Vector.nil)
+def v2 := Vector.cons 8 (Vector.cons 5 (Vector.cons 0 Vector.nil))
+
+-- def add [Add α] : Vector α n → Vector α n → Vector α n
+--   | nil,       nil       => nil
+--   | cons a as, cons b bs => cons (a + b) (add as bs)
+
+
+-- def tailAux (v : Vector α m) : m = n + 1 → Vector α n :=
+--   Vector.casesOn (motive := fun x _ => x = n + 1 → Vector α n) v
+--     (fun h : 0 = n + 1 => Nat.noConfusion h)
+--     (fun (a : α) (m : Nat) (as : Vector α m) =>
+--      fun (h : m + 1 = n + 1) =>
+--        Nat.noConfusion h (fun h1 : m = n => h1 ▸ as))
+
+-- def tail (v : Vector α (n+1)) : Vector α n :=
+--   tailAux v rfl
+
+-- def append: {n m : Nat} → Vector α n → Vector α m → Vector α (n + m)
+--   -- | 0,   nil,       nil       => nil
+--   |  0, _, nil,       k       => k
+--   | cons a as, k => cons a (append as (tail k))
+
+-- #eval add v1 v2
+
+end Vector
+
+-- 5
+inductive Expr where
+  | const : Nat → Expr
+  | var : Nat → Expr
+  | plus : Expr → Expr → Expr
+  | times : Expr → Expr → Expr
+  deriving Repr
+
+open Expr
+
+def sampleExpr : Expr :=
+  plus (times (var 0) (const 7)) (times (const 2) (var 1))
+
+def eval (v : Nat → Nat) : Expr → Nat
+  | const n     => n
+  | var n       => v n
+  | plus e₁ e₂  => (eval v e₁) + (eval v e₂)
+  | times e₁ e₂ => (eval v e₁) * (eval v e₂)
+
+def sampleVal : Nat → Nat
+  | 0 => 5
+  | 1 => 6
+  | _ => 0
+
+-- Try it out. You should get 47 here.
+#eval eval sampleVal sampleExpr
+
+def simpConst : Expr → Expr
+  | plus (const n₁) (const n₂)  => const (n₁ + n₂)
+  | times (const n₁) (const n₂) => const (n₁ * n₂)
+  | e                           => e
+
+#eval simpConst sampleExpr
+
+def fuse : Expr → Expr := sorry
+
+theorem simpConst_eq (v : Nat → Nat)
+        : ∀ e : Expr, eval v (simpConst e) = eval v e :=
+  sorry
+
+theorem fuse_eq (v : Nat → Nat)
+        : ∀ e : Expr, eval v (fuse e) = eval v e :=
+  sorry
+
+
+example : 10 < 5 ∨ 1 > 0 := by
+  decide
+
+example : ¬ (True ∧ False) := by
+  decide
+
+example : 10 * 20 = 200 := by
+  decide
+
+theorem ex : True ∧ 2 = 1+1 := by
+  decide
+
+#print ex
+-- theorem ex : True ∧ 2 = 1 + 1 :=
+-- of_decide_eq_true (Eq.refl true)
+
+#check @of_decide_eq_true
+-- ∀ {p : Prop} [Decidable p], decide p = true → p
+
+#check @decide
+-- (p : Prop) → [Decidable p] → Bool
+
+
+example (a b c : Nat) : a * (b * c) = a * (c * b) := by
+  conv =>
+    -- |- a * (b * c) = a * (c * b)
+    lhs
+    -- |- a * (b * c)
+    congr
+    -- 2 goals : |- a and |- b * c
+    rfl
+    -- |- b * c
+    rw [Nat.mul_comm]
+
+
+#eval 4 = 4
+
+def Set (α : Type u) := α → Prop
+
+namespace Set
+
+def mem (x : α) (a : Set α) := a x
+
+infix:50 (priority := high) "∈" => mem
+
+end Set
+
+theorem tteq : (True ∧ True) = True :=
+  propext (Iff.intro (fun ⟨h, _⟩ => h) (fun h => ⟨h, h⟩))
+
+def val : Nat :=
+  Eq.recOn (motive := fun _ _ => Nat) tteq 0
+
+-- does not reduce to 0
+#reduce val
+
+-- evaluates to 0
+#eval val
